cleanup

src/Iris/Algebra/Heap.lean
@@ -11,101 +11,105 @@ import Iris.Std.Heap
 
 open Iris
 
-section ofe
+section OFE
+
 open OFE
 
-instance Store.instOFE [Store T K V] [OFE V] : OFE T where
+namespace Store
+
+instance instOFE [Store T K V] [OFE V] : OFE T where
   Equiv s0 s1  := get s0 ≡ get s1
   Dist n s0 s1 := get s0 ≡{n}≡ get s1
   dist_eqv     := ⟨fun _ => .of_eq rfl, (·.symm), (·.trans ·)⟩
   equiv_dist   := equiv_dist
   dist_lt      := dist_lt
 
-@[simp] def Store.toMap [Store T K V] [OFE V] : T -n> (K → V) where
+@[simp] def toMap [Store T K V] [OFE V] : T -n> (K → V) where
   f x := get x
   ne.1 {_ _ _} H k := H k
 
-@[simp] def Store.ofMap [Store T K V] [R : RepFunStore T K V] [OFE V] : {f : K → V // R.rep f} -n> T where
+@[simp] def ofMap [Store T K V] [R : RepFunStore T K V] [OFE V] : {f : K → V // R.rep f} -n> T where
   f x := of_fun x
-  ne.1 {_ _ _} H k := by rw [get_of_fun, get_of_fun]; exact H k
+  ne.1 {_ _ _} H k := by simp only [get_of_fun, H k]
 
 instance get_ne [Store T K V] [OFE V] (k : K) : NonExpansive (get · k : T → V) where
   ne {_ _ _} Ht := Ht k
 
 instance [Store T K V] [OFE V] (k : K) : NonExpansive₂ (set · k · : T → V → T) where
   ne {_ _ _} Hv {_ _} Ht k' := by
-    if h : k = k'
-      then rw [get_set_eq h, get_set_eq h]; exact Ht
-      else rw [get_set_ne h, get_set_ne h]; exact Hv k'
+    by_cases h : k = k'
+    · simp [get_set_eq h, Ht]
+    · simp [get_set_ne h, Hv k']
 
-theorem Store.eqv_of_Equiv [OFE V] [Store T K V] {t1 t2 : T} (H : Equiv t1 t2) : t1 ≡ t2 :=
+theorem eqv_of_Equiv [OFE V] [Store T K V] {t1 t2 : T} (H : Store.Equiv t1 t2) : t1 ≡ t2 :=
   (.of_eq <| congrFun H ·)
 
 instance [Heap T K V] [OFE V] (op : V → V → V) [NonExpansive₂ op] :
     NonExpansive₂ (merge (T := T) op) where
-  ne _ {_ _} Ht {_ _} Hs k := by
-    simp only [get_merge]
-    exact NonExpansive₂.ne (Ht k) (Hs k)
+  ne _ {_ _} Ht {_ _} Hs k := by simp only [get_merge]; exact NonExpansive₂.ne (Ht k) (Hs k)
 
 instance [Store T1 K V1] [Store T2 K V2] [OFE V1] [OFE V2] (f : K → V1 → V2)
   [∀ k, NonExpansive (f k)] [HasStoreMap T1 T2 K V1 V2] : NonExpansive (dmap f : T1 → T2) where
   ne _ {_ _} H k := by simp only [get_dmap]; exact NonExpansive.ne (H k)
 
-/-- Project a chain of stores through it's kth coordinate to a chain of values. -/
-def Store.chain [Store T K V] [OFE V] (k : K) (c : Chain T) : Chain V where
+/-- Project a chain of stores through its kth coordinate to a chain of values. -/
+def chain [Store T K V] [OFE V] (k : K) (c : Chain T) : Chain V where
   chain i := get (c i) k
   cauchy Hni := c.cauchy Hni k
 
-theorem Store.chain_get [Store T K V] [OFE V] (k : K) (c : Chain T) :
-    (chain k c) i = get (c i) k := by
-  simp [chain]
+theorem chain_get [Store T K V] [OFE V] (k : K) (c : Chain T) :
+    (chain k c) i = get (c i) k := by simp [chain]
 
-open Store in
+end Store
+
 instance Heap.instCOFE [Heap T K V] [COFE V] : COFE T where
-  compl c := hmap (fun _ => COFE.compl <| c.map ⟨_, get_ne ·⟩) (c 0)
+  compl c := hmap (fun _ => COFE.compl <| c.map ⟨_, Store.get_ne ·⟩) (c 0)
   conv_compl {_ c} k := by
     rw [get_hmap]
     rcases H : get (c.chain 0) k
-    · rw [← chain_get, chain_none_const (c := chain k c) (n := 0) (H▸rfl)]; rfl
+    · simp [← Store.chain_get, chain_none_const (c := Store.chain k c) (n := 0) (H▸rfl)]
     · exact IsCOFE.conv_compl
 
-end ofe
+end OFE
 
-section cmra
+
+section CMRA
 open CMRA
 
 /- ## A CMRA on Heaps -/
 
+namespace Store
+
 variable [Heap T K V] [CMRA V]
 
-@[simp] def Store.op (s1 s2 : T) : T := merge (K := K) CMRA.op s1 s2
-@[simp] def Store.unit : T := empty
-@[simp] def Store.pcore (s : T) : Option T := some <| hmap (fun _ => CMRA.pcore) s
-@[simp] def Store.valid (s : T) : Prop := ∀ k, ✓ (get s k : Option V)
-@[simp] def Store.validN (n : Nat) (s : T) : Prop := ∀ k, ✓{n} (get s k : Option V)
+@[simp] def op (s1 s2 : T) : T := merge (K := K) CMRA.op s1 s2
+@[simp] def unit : T := empty
+@[simp] def pcore (s : T) : Option T := some <| hmap (fun _ => CMRA.pcore) s
+@[simp] def valid (s : T) : Prop := ∀ k, ✓ (get s k : Option V)
+@[simp] def validN (n : Nat) (s : T) : Prop := ∀ k, ✓{n} (get s k : Option V)
 
 theorem lookup_incN {n} {m1 m2 : T} :
-    (∃ (z : T), m2 ≡{n}≡ Store.op m1 z) ↔
+    (∃ (z : T), m2 ≡{n}≡ op m1 z) ↔
     ∀ i, (∃ z, (get m2 i) ≡{n}≡ (get m1 i) • z) := by
   refine ⟨fun ⟨z, Hz⟩ i => ?_, fun H => ?_⟩
   · refine ⟨get z i, ?_⟩
     refine .trans (get_ne i |>.ne Hz) ?_
-    simp only [Store.op, op, optionOp, get_merge]
+    simp only [op, CMRA.op, get_merge]
     cases get m1 i <;> cases get z i <;> simp
   · obtain ⟨f, Hf⟩ := Classical.axiomOfChoice H
     exists hmap (fun k _ => f k) m2
     refine fun i => (Hf i).trans ?_
     specialize Hf i; revert Hf
-    simp [CMRA.op, optionOp, get_merge, get_hmap]
+    simp [CMRA.op, get_merge, get_hmap]
     cases get m2 i <;> cases get m1 i <;> cases f i <;> simp
 
 theorem lookup_inc {m1 m2 : T} :
-    (∃ (z : T), m2 ≡ Store.op m1 z) ↔
-    ∀ i, (∃ z, (Store.get m2 i) ≡ (Store.get m1 i) • z) := by
+    (∃ (z : T), m2 ≡ op m1 z) ↔
+    ∀ i, (∃ z, (get m2 i) ≡ (get m1 i) • z) := by
   refine ⟨fun ⟨z, Hz⟩ i => ?_, fun H => ?_⟩
   · refine ⟨get z i, ?_⟩
     refine .trans (get_ne i |>.eqv Hz) ?_
-    simp only [Store.op, op, optionOp, get_merge]
+    simp only [CMRA.op, op, get_merge]
     cases get m1 i <;> cases get z i <;> simp
   · obtain ⟨f, Hf⟩ := Classical.axiomOfChoice H
     exists hmap (fun k _ => f k) m2
@@ -116,114 +120,115 @@ theorem lookup_inc {m1 m2 : T} :
 
 open OFE in
 instance instStoreCMRA : CMRA T where
-  pcore := Store.pcore
-  op := Store.op
-  ValidN := Store.validN
-  Valid := Store.valid
+  pcore := pcore
+  op := op
+  ValidN := validN
+  Valid := valid
   op_ne.ne _ x1 x2 H i := by
-    specialize H i; revert H; rename_i x _
+    rename_i x _
+    specialize H i; revert H
     simp [get_merge]
     cases get x1 i <;> cases get x2 i <;> cases get x i <;> simp
     apply op_right_dist
   pcore_ne {n x y _} H := by
-    simp only [Store.pcore, Option.some.injEq, exists_eq_left']
+    simp only [pcore, Option.some.injEq, exists_eq_left']
     refine (· ▸ fun k => ?_); specialize H k; revert H
     rw [get_hmap, get_hmap]
-    cases Store.get x k <;> cases Store.get y k <;> simp
+    cases get x k <;> cases get y k <;> simp
     exact (NonExpansive.ne ·)
   validN_ne Hx H k :=
-    validN_ne (NonExpansive.ne (f := (Store.get · k : T → Option V)) Hx) (H k)
+    validN_ne (NonExpansive.ne (f := (get · k : T → Option V)) Hx) (H k)
   valid_iff_validN :=
     ⟨fun H n k => valid_iff_validN.mp (H k) n,
      fun H k => valid_iff_validN.mpr (H · k)⟩
   validN_succ H k := validN_succ (H k)
   validN_op_left {n x1 x2} H k := by
-    refine validN_op_left (y := Store.get x2 k) ?_
+    refine validN_op_left (y := get x2 k) ?_
     specialize H k; revert H
-    simp only [Store.op, get_merge, Option.merge]
-    cases get x1 k <;> cases get x2 k <;> simp [optionOp, op]
+    simp only [op, get_merge, Option.merge]
+    cases get x1 k <;> cases get x2 k <;> simp [optionOp, CMRA.op]
   assoc {x y z} k := by
-    simp only [Store.op, get_merge]
-    cases Store.get x k <;> cases Store.get y k <;> cases Store.get z k <;> simp
+    simp only [op, get_merge]
+    cases get x k <;> cases get y k <;> cases get z k <;> simp
     exact assoc
   comm {x y} k := by
-    simp [Store.op, Heap.get_merge]
-    cases Store.get x k <;> cases Store.get y k <;> simp
+    simp [op, Heap.get_merge]
+    cases get x k <;> cases get y k <;> simp
     exact comm
   pcore_op_left {x cx} H k := by
-    simp only [← Option.getD_some (a := cx) (b := cx), Store.op, get_merge]
-    cases Hcx : Store.get cx k <;> cases hx : Store.get x k <;> simp <;>
-      simp only [Store.pcore, Option.some.injEq] at H
+    simp only [← Option.getD_some (a := cx) (b := cx), op, get_merge]
+    cases Hcx : get cx k <;> cases hx : get x k <;>
+      simp <;>
+      simp only [pcore, Option.some.injEq] at H
     · rw [← H, hmap_unalloc hx] at Hcx
       cases Hcx
     · apply pcore_op_left
       rw [← Hcx, ← H, hmap_alloc hx]
   pcore_idem {x cx} H := by
-    simp only [Store.pcore, Option.some.injEq] at H
-    change (Store.pcore cx |>.getD cx) ≡ cx
+    simp only [pcore, Option.some.injEq] at H
+    change (pcore cx |>.getD cx) ≡ cx
     intro k
     simp [← H, get_hmap]
-    rcases Store.get x k with (_|v) <;> simp
-    cases HY : pcore v; simp
+    rcases get x k with (_|v) <;> simp
+    cases HY : CMRA.pcore v; simp
     exact pcore_idem HY
   pcore_op_mono := by
     apply pcore_op_mono_of_core_op_mono
     rintro x cx y ⟨z, Hz⟩
-    suffices ∃ z, (Store.pcore y |>.getD y) ≡ Store.op (Store.pcore x |>.getD x) z by
+    suffices ∃ z, (pcore y |>.getD y) ≡ op (pcore x |>.getD x) z by
       rintro Hx
-      simp only [Store.pcore, Option.some.injEq, Store.op, exists_eq_left']
+      simp only [pcore, Option.some.injEq, op, exists_eq_left']
       rcases this with ⟨z', Hz'⟩
       exists z'
       refine .trans Hz' (fun i => ?_)
       cases get z' i <;> cases get x i <;> simp_all
     refine lookup_inc.mpr (fun i => ?_)
-    obtain ⟨v', Hv'⟩ : (core (Store.get x i)) ≼ (core (Store.get y i))  := by
+    obtain ⟨v', Hv'⟩ : (core (get x i)) ≼ (core (get y i))  := by
       apply core_mono
       exists get z i
       have Hz := Hz i; revert Hz
       simp [CMRA.op, optionOp, get_merge]
       cases get x i <;> cases get z i <;> simp_all
     exists v'
-    simp_all [core, pcore, optionCore, get_hmap]
+    simp_all [CMRA.core, CMRA.pcore, optionCore, get_hmap]
   extend {n x y1 y2} Hm Heq := by
-    have Hslice i : Store.get x i ≡{n}≡ Store.get y1 i • Store.get y2 i := by
+    have Hslice i : get x i ≡{n}≡ get y1 i • get y2 i := by
       refine (get_ne i |>.ne Heq).trans ?_
       simp [CMRA.op, get_merge, optionOp]
       cases get y1 i <;> cases get y2 i <;> simp
     let extendF (i : K) := CMRA.extend (Hm i) (Hslice i)
     exists hmap (fun k (_ : V) => extendF k |>.fst) y1
     exists hmap (fun k (_ : V) => extendF k |>.snd.fst) y2
-    simp [Store.op]
+    simp [op]
     refine ⟨fun i => ?_, fun i => ?_, fun i => ?_⟩
     all_goals rcases hF : extendF i with ⟨z1, z2, Hm, Hz1, Hz2⟩
     · refine Hm.trans ?_
       simp [get_merge, CMRA.op, optionOp]
       cases z1 <;> cases z2 <;> cases h1 : get y1 i <;> cases h2 : get y2 i <;> simp [h1, h2] at Hz1 Hz2
-      · rw [hmap_unalloc h1, hmap_unalloc h2]; simp
-      · rw [hmap_unalloc h1, hmap_alloc h2, hF]; simp
-      · rw [hmap_alloc h1, hmap_unalloc h2, hF]; simp
+      · simp [hmap_unalloc h1, hmap_unalloc h2]
+      · simp [hmap_unalloc h1, hmap_alloc h2]; rw [hF]; rfl
+      · simp [hmap_alloc h1, hmap_unalloc h2, hF]
       · rw [hmap_alloc h1, hmap_alloc h2, hF]; simp
-    · cases h : Store.get y1 i
+    · cases h : get y1 i
       · rw [hmap_unalloc h]
       · rw [hmap_alloc h, ← h, hF]; exact Hz1
-    · cases h : Store.get y2 i
+    · cases h : get y2 i
       · rw [hmap_unalloc h]
       · rw [hmap_alloc h, ← h, hF]; exact Hz2
 
 instance instStoreUCMRA : UCMRA T where
-  unit := Store.unit
-  unit_valid := by
-    simp [CMRA.Valid, Store.valid, optionValid, Store.unit, get_empty]
-  unit_left_id _ := by
-    simp [CMRA.op, Heap.get_merge, Store.unit, get_empty]
-  pcore_unit _ := by
-    simp [Store.unit, hmap_unalloc get_empty, get_empty]
+  unit := unit
+  unit_valid := by simp [CMRA.Valid, get_empty]
+  unit_left_id _ := by simp [CMRA.op, Heap.get_merge, get_empty]
+  pcore_unit _ := by simp [hmap_unalloc, get_empty]
 
-end cmra
+end Store
+end CMRA
 
 namespace Heap
 
 variable {K V : Type _} [Heap T K V] [CMRA V]
+
 open CMRA Store
 
 theorem validN_get_validN {m : T} (Hv : ✓{n} m) (He : get m i ≡{n}≡ some x) : ✓{n} x := by
@@ -234,14 +239,14 @@ theorem validN_get_validN {m : T} (Hv : ✓{n} m) (He : get m i ≡{n}≡ some x
 theorem valid_get_valid {m : T} (Hv : ✓ m) (He : get m i ≡ some x) : ✓ x :=
   valid_iff_validN.mpr (fun _ => validN_get_validN Hv.validN He.dist)
 
-theorem insert_validN {m : T} (Hx : ✓{n} x) (Hm : ✓{n} m) : ✓{n} (set m i x) := by
+theorem set_validN {m : T} (Hx : ✓{n} x) (Hm : ✓{n} m) : ✓{n} (set m i x) := by
   intro k
   rw [get_set]; split; rename_i He
   · exact Hx
   · apply Hm
 
-theorem insert_valid {m : T} (Hx : ✓ x) (Hm : ✓ m) : ✓ (set m i x) :=
-  valid_iff_validN.mpr (fun _ => insert_validN Hx.validN Hm.validN)
+theorem set_valid {m : T} (Hx : ✓ x) (Hm : ✓ m) : ✓ (set m i x) :=
+  valid_iff_validN.mpr (fun _ => set_validN Hx.validN Hm.validN)
 
 theorem point_valid_iff : ✓ (point i x : T) ↔ ✓ x := by
   refine ⟨fun H => ?_, fun H k => ?_⟩
@@ -267,7 +272,7 @@ theorem set_equiv_point_op_point {m : T} (Hemp : get m i = none) : Equiv (set m 
   simp [CMRA.op, Store.op, get_merge, Option.merge, get_point, get_set]
   split <;> rename_i He
   · rw [← He, Hemp]; cases x <;> rfl
-  · cases (Store.get m k) <;> rfl
+  · cases (get m k) <;> rfl
 
 theorem set_eq_point_op_point [IsoFunStore T K (Option V)] {m : T} (Hemp : get m i = none) :
     set m i x = point i x • m :=
@@ -312,24 +317,27 @@ theorem point_op_point_eq [IsoFunStore T K (Option V)] {i : K} {x y : V} :
 instance {m : T} [∀ x : V, CoreId x] : CoreId m where
   core_id i := by
     rw [get_hmap]
-    cases Store.get m i <;> simp
+    cases get m i <;> simp
     exact core_id
 
 instance [CoreId (x : V)] : CoreId (point (T := T) i (some x)) where
   core_id k := by
     simp [get_hmap, get_point]
     split <;> simp
-    exact  core_id
+    exact core_id
 
 theorem point_incN_iff {m : T} :
     (point (T := T) i (some x)) ≼{n} m ↔ ∃ y, (get m i ≡{n}≡ some y) ∧ some x ≼{n} some y := by
   refine ⟨fun ⟨z, Hz⟩ => ?_, fun ⟨y, Hy, z, Hz⟩ => ?_⟩
-  · specialize Hz i; revert Hz
-    simp only [CMRA.op, Store.op, get_merge, point_get_eq rfl]
-    rcases get z i with (_|v)
-    · intro _
-      exists x
-    · refine (⟨x • v, ·, ?_⟩)
+  · specialize Hz i
+    simp [CMRA.op, Store.op, get_merge, point_get_eq rfl, Option.merge] at Hz
+    rcases He : get z i with (_|v)
+    · exists x
+      simp [He] at Hz
+      exact ⟨Hz, incN_refl (some x)⟩
+    · exists (x • v)
+      simp [He] at Hz
+      refine ⟨Hz, ?_⟩
       exists v
   · exists set m i z
     intro j
@@ -383,16 +391,13 @@ instance [H : Cancelable (some x)] : Cancelable (point (T := T) i (some x)) wher
     specialize Hv j; revert Hv
     specialize He j; revert He
     simp only [CMRA.op, Store.op, get_merge, Option.merge, get_point]
-    if He : i = j
-      then
-        simp_all only [↓reduceIte]
-        intro Hv He
-        cases _ : get m1 j <;> cases _ : get m2 j
-        all_goals apply H.cancelableN
-        all_goals simp_all [CMRA.op, optionOp]
-      else
-        cases get m1 j <;> cases get m2 j
-        all_goals simp_all
+    by_cases He : i = j
+    · simp_all only [↓reduceIte]
+      intro Hv He
+      cases _ : get m1 j <;> cases _ : get m2 j
+      all_goals apply H.cancelableN
+      all_goals simp_all [CMRA.op, optionOp]
+    · cases get m1 j <;> cases get m2 j <;> simp_all
 
 instance {m : T} [Hid : ∀ x : V, IdFree x] [Hc : ∀ x : V, Cancelable x] : Cancelable m where
   cancelableN {n m1 m2} Hv He i := by
@@ -404,19 +409,17 @@ instance {m : T} [Hid : ∀ x : V, IdFree x] [Hc : ∀ x : V, Cancelable x] : Ca
       simp [Heap.get_merge, CMRA.op, Store.op, optionOp]
       cases get m i <;> cases get m1 i <;> cases get m2 i <;> simp_all
 
-theorem insert_op_equiv {m1 m2 : T} :
+theorem set_op_equiv {m1 m2 : T} :
     Equiv ((set (V := Option V) (m1 • m2) i (x • y))) (set m1 i x • set m2 i y) := by
   refine funext fun j => ?_
-  if He : i = j
-    then
-      simp [CMRA.op, get_set_eq He, get_merge, optionOp]
-      cases x <;> cases y <;> simp_all
-    else
-      simp [CMRA.op, get_set_ne (T := T) He, get_merge]
+  by_cases He : i = j
+  · simp [CMRA.op, get_set_eq He, get_merge, optionOp]
+    cases x <;> cases y <;> simp_all
+  · simp [CMRA.op, get_set_ne (T := T) He, get_merge]
 
-theorem insert_op_eq [IsoFunStore T K (Option V)] {m1 m2 : T} :
+theorem set_op_eq [IsoFunStore T K (Option V)] {m1 m2 : T} :
     (set (V := Option V) (m1 • m2) i (x • y)) = (set m1 i x • set m2 i y) :=
-  IsoFunStore.store_eq_of_Equiv insert_op_equiv
+  IsoFunStore.store_eq_of_Equiv set_op_equiv
 
 theorem disjoint_op_equiv_union {m1 m2 : T} (Hd : Set.Disjoint (dom m1) (dom m2)) :
     Equiv (m1 • m2) (union m1 m2) := by
@@ -449,10 +452,11 @@ theorem dom_op_union (m1 m2 : T) : dom (m1 • m2) = Set.Union (dom m1) (dom m2)
   cases get m1 k <;> cases get m2 k <;> simp_all [CMRA.op, dom, Set.Union, get_merge]
 
 theorem inc_dom_inc {m1 m2 : T} (Hinc : m1 ≼ m2) : Set.Included (dom m1) (dom m2) := by
-  intro i; unfold Heap.dom
-  rcases lookup_inc.mp Hinc i with ⟨z, Hz⟩; revert Hz
-  cases get m1 i <;> cases get m2 i <;> cases z <;>
-    simp [CMRA.op, optionOp]
+  intro i
+  unfold Heap.dom
+  rcases lookup_inc.mp Hinc i with ⟨z, Hz⟩
+  revert Hz
+  cases get m1 i <;> cases get m2 i <;> cases z <;> simp [CMRA.op, optionOp]
 
 nonrec instance [HD : CMRA.Discrete V] [Heap T K V] : Discrete T where
   discrete_0 {_ _} H := (OFE.Discrete.discrete_0 <| H ·)
